sml.v
@@ -3,6 +3,9 @@ Require Import Omega.
 Require Import Coq.Lists.List.
 Import ListNotations.
 
+
+Load utils.
+
 Module StackMachine.
 
   Inductive Item : Set :=
@@ -10,13 +13,14 @@ Module StackMachine.
   | item_tuple : list Item -> Item.
 
   Inductive SMProgram : Set :=
+  | sm_end : SMProgram
   | push : nat -> SMProgram -> SMProgram
   | pop : SMProgram -> SMProgram
   | get : nat -> SMProgram -> SMProgram
   (*| rotate : nat -> SMProgram -> SMProgram *)
   | pack : nat -> SMProgram -> SMProgram
   | unpack : SMProgram -> SMProgram
-  | call : SMProgram -> SMProgram
+  | jump : SMProgram
   | out : SMProgram -> SMProgram.
 
 
@@ -26,7 +30,6 @@ Module StackMachine.
     state (ast: SMProgram)
           (fn_table: list SMProgram)
           (stack: Stack)
-          (input: list nat)
           (output: list nat).
 
   Definition failsafe_tl {A: Type} (l: list A) :=
@@ -34,8 +37,6 @@ Module StackMachine.
     | [] => []
     | _ :: tl => tl
     end.
-
-
 
   (* Monads ftw! *)
   Definition bind {A B : Type} (a: option A) (f : A -> option B) :=
@@ -52,7 +53,7 @@ Module StackMachine.
     | _ :: tl => Some tl
     end.
 
-  Definition hd_error {A} (l : list A) : option (list A) :=
+  Definition hd_error {A} (l : list A) : option A :=
     match l with
     | [] => None
     | hd :: _ => Some hd
@@ -91,26 +92,54 @@ Module StackMachine.
     (stack_pack n s) = Some s' ->
     (stack_pack n s) >>= stack_unpack = Some s.
   Proof.
-    admit.
   Admitted.
 
   Function sm_step (s: SMState): option SMState :=
     match s with
-    | state smp fn_table stack input output =>
+    | state smp fn_table stack output =>
       let state_from_stack (smp': SMProgram) (stack : Stack) :=
-        Some (state smp' fn_table stack input output)
+        Some (state smp' fn_table stack output)
       in match smp with
+      | sm_end => None
       | push n smp' => state_from_stack smp' ((item_nat n) :: stack)
       | pop smp'=> (tl_error stack) >>= (state_from_stack smp')
       | get n smp' =>
         let new_stack := (nth_error stack n) >>= (fun a => Some (a :: stack)) 
         in new_stack >>= (state_from_stack smp')
       | pack n smp' => (stack_pack n stack) >>= (state_from_stack smp')
-      | unpack n smp' => (stack_unpack stack) >>= (state_from_stack smp')
-      | call smp' => match stack with
+      | unpack smp' => (stack_unpack stack) >>= (state_from_stack smp')
+      | jump => match stack with
         | (item_nat id) :: tl => (nth_error fn_table id) >>= (fun smp =>
-          Some (state smp fn_table tl input output))
+          Some (state smp fn_table tl output))
         | _ => None
         end
+      | out smp' => match stack with
+        | (item_nat o) :: _ => Some o
+        | _ => None
+        end
+        >>= (fun o => Some (state smp' fn_table stack (o :: output)))
       end
     end.
+
+  (* TODO: Abstract the functions below along with the stuff in bftape.v *)
+  Definition exec_output (state: SMState): list nat :=
+    match state with state _ _ _ output => output end.
+
+  Definition exec_init (fn_table: list SMProgram) : option SMState :=
+    match fn_table with
+    | smp :: _ => Some (state smp fn_table [] [])
+    | [] => None
+    end.
+
+  Definition interpret (fn_table: list SMProgram) (fuel: nat): option (list nat) :=
+    (exec_init fn_table) >>= (fun state => Utils.run sm_step state exec_output fuel). 
+
+  Example push_simple:
+    interpret [push 3 (out sm_end)] 20 = Some [3].
+  Proof. auto. Qed.
+
+  Example jump_simple:
+    interpret [push 1 (out jump); push 3 (out sm_end)] 20 = Some [3; 1].
+  Proof. auto. Qed.
+
+End StackMachine.
