utils.v
@@ -1,0 +1,19 @@
+Require Import Arith.
+Require Import Omega.
+Require Import Coq.Lists.List.
+Import ListNotations.
+
+Module Utils.
+  (* TODO: Use N as fuel with {measure N.to_nat fuel} *)
+  Function run {State: Type} (step: State -> option State)
+           (state: State) (output: State -> list nat)
+           (fuel: nat): option (list nat) :=
+    match fuel with
+    | 0 => None
+    | S f =>
+      match step state with
+      | None => Some (output state)
+      | Some state' => run step state' output f
+      end
+    end.
+End Utils.
